theories/cancellation/CancelSpawn.v
@@ -1,12 +1,9 @@
-(* Require Import CRIS.
+Require Import CRIS.
 Require Import LMod LModTr GSim GSimFacts GSimTactics.
 Require Import MInline MInlineIntro MInlineElim ElimRel.
 
-Lemma cancel_spawn `{_crisG: !crisG Γ Σ α β τ _S _I, _concG: !concG} md sp fn args img0 :
-  (img0 = false → fspec_imply (fspec_flat (sp fn)) fspec_trivial) →
-  CANCEL_GOAL md sp
-    (NativeSpawnE fn args)
-    (HoareSpawnE fn args ((if img0 then sp else sp_none) fn)).
+Lemma cancel_spawn `{_crisG: !crisG Γ Σ α β τ _S _I, _concG: !concG} md sp fn args :
+  CANCEL_GOAL md sp (NativeSpawnE fn args) (HoareSpawnE fn args (sp fn)).
 Proof.
   r; i. assert (VP0:=VP). destruct VP0 as [VP1 VP2]. r in VP1.
   rewrite /sp_from /to_sp in VP1. setoid_rewrite alist_find_map_snd in VP1.
@@ -14,42 +11,59 @@ Proof.
   rewrite !alist_find_map_snd.
   destruct (alist_find (Some fn) (SMod.fnsems md)) eqn: FIND; rewrite !FIND; cycle 1.
   { s. zstep_l. }
-  destruct f as [[[img msk] scp] [fspo bd]].
+  destruct f as [[msk scp] [fspo bd]].
   assert (WFSCP: incl scp (SMod.scopes md)).
   { etrans; [|apply SMod.well_scoped_fns].
     rewrite /fnsems_scopes. erewrite FIND. refl.
   }
 
-  destruct ((if img0 then sp else sp_none) fn) eqn: E; s.
+  destruct (sp fn) eqn: E; s; cycle 1.
+  { des. specialize (VP2 fn). rewrite E /sp_from /to_sp alist_find_map_snd FIND /= in VP2.
+    destruct fspo; ss. destruct f; ss. r in VP0. hexploit VP0; eauto. i; ss. }
   { (* the spawnee has a non-trivial spec *)
     destruct f.
     { ired. zstep_r. }
+    destruct fspo; cycle 1.
+    { des. r in VP0. hexploit VP0; eauto; i; ss. }
+    destruct f.
+    { des. specialize (VP2 fn). rewrite E /sp_from /to_sp alist_find_map_snd FIND // in VP2. }
     ired. ziter_l. zstep_l.
     do 2 zstep_r.
     ziter_r; zstep_r.
     ziter_r; do 2 zstep_r.
     ziter_r; zstep_r.
     ziter_r; zstep_r.
-    (* rewrite !alist_find_map_snd FIND. ired. *)
-    (* ziter_r; do 2 zstep_r. *)
-    (* ziter_r; do 2 zstep_r. *)
-    (* ziter_r; zstep_r. ziter_r; zstep_r. *)
-    (* ziter_r; zstep_r. ziter_r; zstep_r. *)
     rewrite !alist_find_map_snd FIND /=. ired.
     ziter_r; zstep_r.
     ziter_r; zstep_r.
     ziter_r; zstep_r.
-    exists r_t. zstep_r.
+    rewrite YieldToken_gen in RS.
+    hexploit (Own_bupd_split).
+    { iIntros "S". iPoseProof (RS with "S") as ">(D & T & TA & YA & Y)".
+      iModIntro. iCombine "D TA YA" as "P". iCombine "T Y" as "Q".
+      iSplitL "P"; [iApply "P"|iApply "Q"]. }
+    { eauto. }
+    intros [r_t1 [r_t2 [Hr_t [Hr_t1 Hr_t2]]]].
+    exists r_t2. zstep_r.
     ziter_r; zstep_r.
-    eexists.
+    assert (RES: ✓ r_t2 ∧ (Own r_t2 ⊢ |==> YIELD (length tgts) ∗ Own r_t)).
+    { split; eauto.
+      { eapply Own_wand_valid; [iIntros "S"; iMod (Hr_t with "S") as "[_ $]"; done|eauto]. }
+      { rewrite Hr_t2 EQLEN2 EQLEN. iIntros "[$ $]"; done. }
+    }
+    exists RES.
     zstep_r.
+    do 4 (ziter_r; zstep_r).
+    ziter_r; do 2 zstep_r.
+    ziter_r; do 2 zstep_r.
+    do 3 (ziter_r; zstep_r).
     zprogress. gbase.
     des; hexploit (Own_bupd_split); et.
-    { eapply Own_wand_valid; [iIntros "X"; iMod (RS with "X") as "[? $]"; done|]; done. }
-    intros [r_t1 [r_t2 [Hr_t [Hr_t1 Hr_t2]]]].
+    (* { eapply Own_wand_valid; [iIntros "X"; iMod (Hr_t with "X") as "[? $]"; done|]; done. } *)
+    intros [r_t3 [r_t4 [Hr_t3 [Hr_t4 Hr_t5]]]].
     eapply CIH; eauto.
     { rewrite -!insert_app_l; try lia.
-      instantiate (1:=<[cid:=ε]>(rs_diff ++ [r_t1])).
+      instantiate (1:=<[cid:=ε]>(rs_diff ++ [r_t3])).
       econs; first (rewrite !length_insert !length_app /=; lia).
       econs; first (rewrite !length_insert !length_app /=; lia).
       intros i ???; destruct (decide (i = cid)).
@@ -65,23 +79,26 @@ Proof.
       subst; rewrite list_lookup_length EQLEN list_lookup_length -EQLEN -EQLEN2 list_lookup_length.
       do 3 (intros INV; inv INV).
 
-      rewrite /ModTr.trans_ktree !sandbox_inline_commute /SB.sandbox_body //=.
-      rewrite (MIRed_HoareFun _ _ fn) //= if_simpl SBRed.tau MIRed.tau.
-      hexploit (VP1 fn); rewrite FIND /=; revert E; destruct img0; ss; intros ->; ss; intros Himp.
-      hexploit (Himp x); intros [x' [PRE ?]].
+      rewrite /ModTr.trans_ktree !sandbox_inline_commute /SB.sandbox_body; try by eauto.
+      rewrite /SModTr.trans_ktree /SModTr.trans_body.
+      replace (SModTr.HoareFun (Some _)) with (Seal.sealing "temp" (SModTr.HoareFun (Some (fspec_spawn precond0 postcond0)))); cycle 1.
+      { unseal "temp". refl. }
+      ss. unseal "temp".
+      rewrite (@MIRed_HoareFun _ _ _ _ _ _ _ _ _ md sp msk scp bd (Some (fspec_spawn precond0 postcond0)) x3 fn meta0 precond0 postcond0); eauto.
+      rewrite SBRed.tau MIRed.tau.
+      hexploit (VP1 fn); rewrite FIND /=; revert E; intros ->; ss; intros Himp.
+      hexploit (Himp (length tgts) x); intros [x' [PRE ?]].
       eapply thread_rel_spawn; eauto.
       { destruct rs_diff; ss. }
-      { destruct fspo; ss.
-        { iIntros "X //". iApply PRE; iApply Hr_t1; done. }
-        { iIntros "X //". iPoseProof (Hr_t1 with "X") as "X".
-          iMod (PRE with "X") as "%"; done.
-        }
+      { iIntros "X //". iPoseProof (Hr_t4 with "X") as "X".
+        rewrite EQLEN2 EQLEN. unfold FSpec.precond, FSpec.postcond in *.
+        iMod (PRE with "X") as "X"; done.
       }
       { ss; eapply elim_rel_cancel; eauto. }
     }
     rewrite insert_app_l; last lia.
-    rewrite list_insert_id // big_sepL_app /= right_id RS Hr_t Hr_t2.
-    iIntros "> [$ > [$ $]]"; done.
+    rewrite Hr_t Hr_t1 Hr_t3 Hr_t5 list_insert_id // big_sepL_app /= right_id last_length.
+    iIntros ">(($ & $) & >[$ $])"; done.
   }
       (* Experimental *)
       (* rewrite interpV_bind.
@@ -116,56 +133,55 @@ Proof.
     rewrite list_insert_id // big_sepL_app /= right_id RS Hr_t Hr_t2.
     iIntros "> [$ > [$ $]]"; done.
   } *)
-  { (* fn has a trivial spec in sp *)
-    ired. zstep_r.
-    ziter_l; zstep_l.
-    rewrite !alist_find_map_snd FIND /=; ired.
-    ziter_r; zstep_r.
-    zprogress. gbase.
-    eapply CIH.
-    { rewrite -!insert_app_l; try lia.
-      instantiate (1:=<[cid:=ε]>(rs_diff ++ [ε])).
-      econs; first (rewrite !length_insert !length_app /=; lia).
-      econs; first (rewrite !length_insert !length_app /=; lia).
-      intros i ???; destruct (decide (i = cid)).
-      { subst; rewrite ?list_lookup_insert; try (rewrite length_app /=; lia).
-        do 3 (intros INV; inv INV).
-        econs; eauto. rewrite -EQLEN; eapply KTR.
-      }
-      rewrite !list_lookup_insert_ne //.
-      destruct (decide (i < length srcs)).
-      { rewrite !lookup_app_l; try lia. ii; eapply REL; eauto. }
-      destruct (decide (i = length srcs)); cycle 1.
-      { rewrite ?lookup_ge_None_2; ss; rewrite ?length_app /=; lia. }
-      subst; rewrite list_lookup_length EQLEN list_lookup_length -EQLEN -EQLEN2 list_lookup_length.
-      do 3 (intros INV; inv INV).
-      rewrite /ModTr.trans_ktree !sandbox_inline_commute /SB.sandbox_body //=.
-      rewrite (MIRed_HoareFun _ _ fn) //= if_simpl SBRed.tau MIRed.tau.
-      (* econs; eauto; cycle 1.
-      { rewrite bind_ret_r //. } *)
-      (* rewrite !sandbox_inline_commute //.
-      rewrite !if_simpl /SB.sandbox_body /= (MIRed_HoareFun _ _ fn) //. *)
+  (* { (* fn has a trivial spec in sp *) *)
+  (*   ired. zstep_r. *)
+  (*   ziter_l; zstep_l. *)
+  (*   rewrite !alist_find_map_snd FIND /=; ired. *)
+  (*   ziter_r; zstep_r. *)
+  (*   zprogress. gbase. *)
+  (*   eapply CIH. *)
+  (*   { rewrite -!insert_app_l; try lia. *)
+  (*     instantiate (1:=<[cid:=ε]>(rs_diff ++ [ε])). *)
+  (*     econs; first (rewrite !length_insert !length_app /=; lia). *)
+  (*     econs; first (rewrite !length_insert !length_app /=; lia). *)
+  (*     intros i ???; destruct (decide (i = cid)). *)
+  (*     { subst; rewrite ?list_lookup_insert; try (rewrite length_app /=; lia). *)
+  (*       do 3 (intros INV; inv INV). *)
+  (*       econs; eauto. rewrite -EQLEN; eapply KTR. *)
+  (*     } *)
+  (*     rewrite !list_lookup_insert_ne //. *)
+  (*     destruct (decide (i < length srcs)). *)
+  (*     { rewrite !lookup_app_l; try lia. ii; eapply REL; eauto. } *)
+  (*     destruct (decide (i = length srcs)); cycle 1. *)
+  (*     { rewrite ?lookup_ge_None_2; ss; rewrite ?length_app /=; lia. } *)
+  (*     subst; rewrite list_lookup_length EQLEN list_lookup_length -EQLEN -EQLEN2 list_lookup_length. *)
+  (*     do 3 (intros INV; inv INV). *)
+  (*     rewrite /ModTr.trans_ktree !sandbox_inline_commute /SB.sandbox_body //=. *)
+  (*     rewrite (MIRed_HoareFun _ _ fn) //= if_simpl SBRed.tau MIRed.tau. *)
+  (*     (* econs; eauto; cycle 1. *)
+  (*     { rewrite bind_ret_r //. } *) *)
+  (*     (* rewrite !sandbox_inline_commute //. *)
+  (*     rewrite !if_simpl /SB.sandbox_body /= (MIRed_HoareFun _ _ fn) //. *) *)
 
-      assert (Himpl : fspec_imply (fspec_flat fspo) fspec_trivial).
-      { hexploit (VP1 fn); rewrite FIND /=; intros Himpl.
-        destruct img0.
-        { rewrite E in Himpl; ss. }
-        { etrans; eauto. }
-      }
-      hexploit (Himpl ()); intros [? [PRE ?]].
-      eapply thread_rel_spawn; eauto.
-      { destruct rs_diff; ss. }
-      { destruct fspo; ss.
-        { iIntros "X //". iApply PRE; done. }
-        { iIntros "X //". }
-      }
-      { ss; eapply elim_rel_cancel; eauto. }
-    }
-    { eauto. }
-    { rewrite insert_app_l; last lia.
-      rewrite list_insert_id // big_sepL_app /= right_id RS.
-      iIntros "> [$ $] !>"; iApply Own_unit.
-    }
-  }
+  (*     assert (Himpl : fspec_imply (fspec_flat fspo) fspec_trivial). *)
+  (*     { hexploit (VP1 fn); rewrite FIND /=; intros Himpl. *)
+  (*       destruct img0. *)
+  (*       { rewrite E in Himpl; ss. } *)
+  (*       { etrans; eauto. } *)
+  (*     } *)
+  (*     hexploit (Himpl ()); intros [? [PRE ?]]. *)
+  (*     eapply thread_rel_spawn; eauto. *)
+  (*     { destruct rs_diff; ss. } *)
+  (*     { destruct fspo; ss. *)
+  (*       { iIntros "X //". iApply PRE; done. } *)
+  (*       { iIntros "X //". } *)
+  (*     } *)
+  (*     { ss; eapply elim_rel_cancel; eauto. } *)
+  (*   } *)
+  (*   { eauto. } *)
+  (*   { rewrite insert_app_l; last lia. *)
+  (*     rewrite list_insert_id // big_sepL_app /= right_id RS. *)
+  (*     iIntros "> [$ $] !>"; iApply Own_unit. *)
+  (*   } *)
+  (* } *)
 (*SLOW*)Qed.
-*)
